Helpers.thy
@@ -2,9 +2,12 @@ theory Helpers
   imports Utils Types Config Invariants "HOL-Library.Monad_Syntax"
 begin
 
+definition compute_start_slot_at_epoch :: "Config \<Rightarrow> Epoch \<Rightarrow> Slot" where
+  "compute_start_slot_at_epoch c e \<equiv> Slot (the (epoch_to_u64 e .* SLOTS_PER_EPOCH c))"
+
 definition get_current_epoch :: "Config \<Rightarrow> BeaconState \<Rightarrow> Epoch" where
   "get_current_epoch c state \<equiv>
-    Epoch (the ((slot_to_u64 (slot state) \\ SLOTS_PER_EPOCH c)))"
+    Epoch (the ((slot_to_u64 (slot_f state) \\ SLOTS_PER_EPOCH c)))"
 
 definition get_previous_epoch :: "Config \<Rightarrow> BeaconState \<Rightarrow> Epoch" where
   "get_previous_epoch c state \<equiv>
@@ -16,11 +19,11 @@ definition get_previous_epoch :: "Config \<Rightarrow> BeaconState \<Rightarrow>
 
 definition is_active_validator :: "Validator \<Rightarrow> Epoch \<Rightarrow> bool" where
   "is_active_validator validator e \<equiv>
-    activation_epoch validator \<le> e \<and> e < exit_epoch validator"
+    activation_epoch_f validator \<le> e \<and> e < exit_epoch_f validator"
 
 definition get_active_validator_indices :: "BeaconState \<Rightarrow> Epoch \<Rightarrow> u64 list" where
   "get_active_validator_indices state e \<equiv>
-    [i. (i, v) \<leftarrow> enumerate (list_inner (validators state)), is_active_validator v e]"
+    [i. (i, v) \<leftarrow> enumerate (list_inner (validators_f state)), is_active_validator v e]"
 
 definition has_flag :: "ParticipationFlags \<Rightarrow> nat \<Rightarrow> bool" where
   "has_flag flags flag_index \<equiv>
@@ -34,22 +37,24 @@ where
     let current_epoch = get_current_epoch c state;
     _ \<leftarrow> assert (e = previous_epoch \<or> e = current_epoch);
     let epoch_participation = (if e = current_epoch then
-      current_epoch_participation state
+      current_epoch_participation_f state
     else
-      previous_epoch_participation state);
+      previous_epoch_participation_f state);
     let active_validator_indices = get_active_validator_indices state e;
     let participating_indices = [
-      i. i \<leftarrow> active_validator_indices, has_flag (list_index epoch_participation i) flag_index
+      i.
+      i \<leftarrow> active_validator_indices,
+      has_flag (unsafe_list_index epoch_participation i) flag_index
     ];
     Some (
       set (
-        filter (\<lambda>index. \<not> slashed (list_index (validators state) index))
+        filter (\<lambda>index. \<not> slashed_f (unsafe_list_index (validators_f state) index))
                participating_indices))
   }"
 
 definition get_total_balance :: "Config \<Rightarrow> BeaconState \<Rightarrow> u64 set \<Rightarrow> u64 option" where
   "get_total_balance c state indices \<equiv> do {
-    total \<leftarrow> safe_sum ((\<lambda>i. effective_balance (list_index (validators state) i)) ` indices);
+    total \<leftarrow> safe_sum ((\<lambda>i. effective_balance_f (unsafe_list_index (validators_f state) i)) ` indices);
     Some (max (EFFECTIVE_BALANCE_INCREMENT c) total)
   }"
 
@@ -57,5 +62,17 @@ definition get_total_active_balance :: "Config \<Rightarrow> BeaconState \<Right
   "get_total_active_balance c state \<equiv>
     get_total_balance c state
                       (set (get_active_validator_indices state (get_current_epoch c state)))"
+
+definition get_block_root_at_slot :: "Config \<Rightarrow> BeaconState \<Rightarrow> Slot \<Rightarrow> Hash256 option" where
+  "get_block_root_at_slot c state slot \<equiv> do {
+    upper_limit \<leftarrow> slot .+ Slot (SLOTS_PER_HISTORICAL_ROOT c);
+    _ \<leftarrow> assert (slot < slot_f state \<and> slot_f state \<le> upper_limit);
+    i \<leftarrow> slot_to_u64 slot .% SLOTS_PER_HISTORICAL_ROOT c;
+    vector_index (block_roots_f state) i
+  }"
+
+definition get_block_root :: "Config \<Rightarrow> BeaconState \<Rightarrow> Epoch \<Rightarrow> Hash256 option" where
+  "get_block_root c state epoch \<equiv>
+    get_block_root_at_slot c state (compute_start_slot_at_epoch c epoch)"
 
 end
