Invariants.thy
@@ -37,39 +37,42 @@ definition valid_version :: "Version \<Rightarrow> bool" where
 
 definition valid_fork :: "Fork \<Rightarrow> bool" where
   "valid_fork f \<equiv>
-    valid_version (previous_version f) \<and>
-    valid_version (current_version f) \<and>
-    valid_epoch (Fork.epoch f)"
+    valid_version (previous_version_f f) \<and>
+    valid_version (current_version_f f) \<and>
+    valid_epoch (Fork.epoch_f f)"
 
 definition valid_beacon_block_header :: "BeaconBlockHeader \<Rightarrow> bool" where
   "valid_beacon_block_header header \<equiv>
-    valid_slot (BeaconBlockHeader.slot header) \<and>
-    valid_u64 (proposer_index header) \<and>
-    valid_hash256 (parent_root header) \<and>
-    valid_hash256 (state_root header) \<and>
-    valid_hash256 (body_root header)"
+    valid_slot (BeaconBlockHeader.slot_f header) \<and>
+    valid_u64 (proposer_index_f header) \<and>
+    valid_hash256 (parent_root_f header) \<and>
+    valid_hash256 (state_root_f header) \<and>
+    valid_hash256 (body_root_f header)"
 
 definition valid_eth1_data :: "Eth1Data \<Rightarrow> bool" where
   "valid_eth1_data data \<equiv>
-    valid_hash256 (deposit_root data) \<and>
-    valid_u64 (deposit_count data) \<and>
-    valid_hash256 (block_hash data)"
+    valid_hash256 (deposit_root_f data) \<and>
+    valid_u64 (deposit_count_f data) \<and>
+    valid_hash256 (block_hash_f data)"
 
 definition valid_validator :: "Validator \<Rightarrow> bool" where
   "valid_validator v \<equiv>
-    valid_public_key (pubkey v) \<and>
-    valid_hash256 (withdrawal_credentials v) \<and>
-    valid_u64 (effective_balance v) \<and>
-    valid_epoch (activation_eligibility_epoch v) \<and>
-    valid_epoch (activation_epoch v) \<and>
-    valid_epoch (exit_epoch v) \<and>
-    valid_epoch (withdrawable_epoch v)"
+    valid_public_key (pubkey_f v) \<and>
+    valid_hash256 (withdrawal_credentials_f v) \<and>
+    valid_u64 (effective_balance_f v) \<and>
+    valid_epoch (activation_eligibility_epoch_f v) \<and>
+    valid_epoch (activation_epoch_f v) \<and>
+    valid_epoch (exit_epoch_f v) \<and>
+    valid_epoch (withdrawable_epoch_f v)"
+
+primrec bitvector_inner :: "Bitvector \<Rightarrow> bool list" where
+  "bitvector_inner (Bitvector bools) = bools"
 
 definition valid_bitvector :: "u64 \<Rightarrow> Bitvector \<Rightarrow> bool" where
   "valid_bitvector n v \<equiv> case v of Bitvector bools \<Rightarrow> length bools = u64_to_nat n"
 
 definition valid_checkpoint :: "Checkpoint \<Rightarrow> bool" where
-  "valid_checkpoint c \<equiv> valid_epoch (Checkpoint.epoch c) \<and> valid_hash256 (Checkpoint.root c)"
+  "valid_checkpoint c \<equiv> valid_epoch (Checkpoint.epoch_f c) \<and> valid_hash256 (Checkpoint.root_f c)"
 
 definition valid_participation_flags :: "ParticipationFlags \<Rightarrow> bool" where
   "valid_participation_flags flags \<equiv>
@@ -77,36 +80,36 @@ definition valid_participation_flags :: "ParticipationFlags \<Rightarrow> bool" 
 
 definition valid_sync_committee :: "Config \<Rightarrow> SyncCommittee \<Rightarrow> bool" where
   "valid_sync_committee c sync_committee \<equiv>
-    valid_vector valid_public_key (SYNC_COMMITTEE_SIZE c) (pubkeys sync_committee) \<and>
-    valid_public_key (aggregate_pubkey sync_committee)"
+    valid_vector valid_public_key (SYNC_COMMITTEE_SIZE c) (pubkeys_f sync_committee) \<and>
+    valid_public_key (aggregate_pubkey_f sync_committee)"
 
 definition valid_beacon_state :: "Config \<Rightarrow> BeaconState \<Rightarrow> bool" where
   "valid_beacon_state c state \<equiv>
-    valid_u64 (genesis_time state) \<and>
-    valid_hash256 (genesis_validators_root state) \<and>
-    valid_slot (slot state) \<and>
-    valid_fork (fork state) \<and>
-    valid_beacon_block_header (latest_block_header state) \<and>
-    valid_vector valid_hash256 (SLOTS_PER_HISTORICAL_ROOT c) (block_roots state) \<and>
-    valid_vector valid_hash256 (SLOTS_PER_HISTORICAL_ROOT c) (state_roots state) \<and>
-    valid_list valid_hash256 (HISTORICAL_ROOTS_LIMIT c) (historical_roots state) \<and>
-    valid_eth1_data (eth1_data state) \<and>
-    valid_list valid_eth1_data (SLOTS_PER_ETH1_VOTING_PERIOD c) (eth1_data_votes state) \<and>
-    valid_u64 (eth1_deposit_index state) \<and>
-    valid_list valid_validator (VALIDATOR_REGISTRY_LIMIT c) (validators state) \<and>
-    valid_list valid_u64 (VALIDATOR_REGISTRY_LIMIT c) (balances state) \<and>
-    valid_vector valid_hash256 (EPOCHS_PER_HISTORICAL_VECTOR c) (randao_mixes state) \<and>
-    valid_vector valid_u64 (EPOCHS_PER_SLASHINGS_VECTOR c) (slashings state) \<and>
+    valid_u64 (genesis_time_f state) \<and>
+    valid_hash256 (genesis_validators_root_f state) \<and>
+    valid_slot (slot_f state) \<and>
+    valid_fork (fork_f state) \<and>
+    valid_beacon_block_header (latest_block_header_f state) \<and>
+    valid_vector valid_hash256 (SLOTS_PER_HISTORICAL_ROOT c) (block_roots_f state) \<and>
+    valid_vector valid_hash256 (SLOTS_PER_HISTORICAL_ROOT c) (state_roots_f state) \<and>
+    valid_list valid_hash256 (HISTORICAL_ROOTS_LIMIT c) (historical_roots_f state) \<and>
+    valid_eth1_data (eth1_data_f state) \<and>
+    valid_list valid_eth1_data (SLOTS_PER_ETH1_VOTING_PERIOD c) (eth1_data_votes_f state) \<and>
+    valid_u64 (eth1_deposit_index_f state) \<and>
+    valid_list valid_validator (VALIDATOR_REGISTRY_LIMIT c) (validators_f state) \<and>
+    valid_list valid_u64 (VALIDATOR_REGISTRY_LIMIT c) (balances_f state) \<and>
+    valid_vector valid_hash256 (EPOCHS_PER_HISTORICAL_VECTOR c) (randao_mixes_f state) \<and>
+    valid_vector valid_u64 (EPOCHS_PER_SLASHINGS_VECTOR c) (slashings_f state) \<and>
     valid_list valid_participation_flags (VALIDATOR_REGISTRY_LIMIT c)
-               (previous_epoch_participation state) \<and>
+               (previous_epoch_participation_f state) \<and>
     valid_list valid_participation_flags (VALIDATOR_REGISTRY_LIMIT c)
-               (current_epoch_participation state) \<and>
-    valid_bitvector (JUSTIFICATION_BITS_LENGTH c) (justification_bits state) \<and>
-    valid_checkpoint (previous_justified_checkpoint state) \<and>
-    valid_checkpoint (current_justified_checkpoint state) \<and>
-    valid_checkpoint (finalized_checkpoint state) \<and>
-    valid_list valid_u64 (VALIDATOR_REGISTRY_LIMIT c) (inactivity_scores state) \<and>
-    valid_sync_committee c (current_sync_committee state) \<and>
-    valid_sync_committee c (next_sync_committee state)"
+               (current_epoch_participation_f state) \<and>
+    valid_bitvector (JUSTIFICATION_BITS_LENGTH c) (justification_bits_f state) \<and>
+    valid_checkpoint (previous_justified_checkpoint_f state) \<and>
+    valid_checkpoint (current_justified_checkpoint_f state) \<and>
+    valid_checkpoint (finalized_checkpoint_f state) \<and>
+    valid_list valid_u64 (VALIDATOR_REGISTRY_LIMIT c) (inactivity_scores_f state) \<and>
+    valid_sync_committee c (current_sync_committee_f state) \<and>
+    valid_sync_committee c (next_sync_committee_f state)"
 
 end
