Types.thy
@@ -2,9 +2,12 @@ theory Types
   imports Main Unsigned
 begin
 
-datatype Hash256 = Hash256 "u8 list"
+(*
+ * We use names ending in _f for all record fields to prevent the unadorned name becoming
+ * unusable. See: https://isabelle.in.tum.de/dist/library/Doc/Tutorial/Records.html
+*)
 
-(* FIXME: enforce length at type level? *)
+datatype Hash256 = Hash256 "u8 list"
 datatype 'a Vector = Vector "'a list"
 datatype 'a List = List "'a list"
 
@@ -15,66 +18,66 @@ datatype PublicKey = PublicKey "u8 list"
 datatype Version = Version "u8 list"
 
 record Fork =
-  previous_version :: Version
-  current_version :: Version
-  epoch :: Epoch
+  previous_version_f :: Version
+  current_version_f :: Version
+  epoch_f :: Epoch
 
 record BeaconBlockHeader =
-  slot :: Slot
-  proposer_index :: u64
-  parent_root :: Hash256
-  state_root :: Hash256
-  body_root :: Hash256
+  slot_f :: Slot
+  proposer_index_f :: u64
+  parent_root_f :: Hash256
+  state_root_f :: Hash256
+  body_root_f :: Hash256
 
 record Eth1Data =
-  deposit_root :: Hash256
-  deposit_count :: u64
-  block_hash :: Hash256
+  deposit_root_f :: Hash256
+  deposit_count_f :: u64
+  block_hash_f :: Hash256
 
 record Validator =
-  pubkey :: PublicKey
-  withdrawal_credentials :: Hash256
-  effective_balance :: u64
-  slashed :: bool
-  activation_eligibility_epoch :: Epoch
-  activation_epoch :: Epoch
-  exit_epoch :: Epoch
-  withdrawable_epoch :: Epoch
+  pubkey_f :: PublicKey
+  withdrawal_credentials_f :: Hash256
+  effective_balance_f :: u64
+  slashed_f :: bool
+  activation_eligibility_epoch_f :: Epoch
+  activation_epoch_f :: Epoch
+  exit_epoch_f :: Epoch
+  withdrawable_epoch_f :: Epoch
 
 datatype ParticipationFlags = ParticipationFlags "bool list"
 
 record Checkpoint =
-  epoch :: Epoch
-  root :: Hash256
+  epoch_f :: Epoch
+  root_f :: Hash256
 
 record SyncCommittee =
-  pubkeys :: "PublicKey Vector"
-  aggregate_pubkey :: PublicKey
+  pubkeys_f :: "PublicKey Vector"
+  aggregate_pubkey_f :: PublicKey
 
 record BeaconState =
-  genesis_time :: u64
-  genesis_validators_root :: Hash256
-  slot :: Slot
-  fork :: Fork
-  latest_block_header :: BeaconBlockHeader
-  block_roots :: "Hash256 Vector"
-  state_roots :: "Hash256 Vector"
-  historical_roots :: "Hash256 List"
-  eth1_data :: Eth1Data
-  eth1_data_votes :: "Eth1Data List"
-  eth1_deposit_index :: u64
-  validators :: "Validator List"
-  balances :: "u64 List"
-  randao_mixes :: "Hash256 Vector"
-  slashings :: "u64 Vector"
-  previous_epoch_participation :: "ParticipationFlags List"
-  current_epoch_participation :: "ParticipationFlags List"
-  justification_bits :: Bitvector
-  previous_justified_checkpoint :: Checkpoint
-  current_justified_checkpoint :: Checkpoint
-  finalized_checkpoint :: Checkpoint
-  inactivity_scores :: "u64 List"
-  current_sync_committee :: SyncCommittee
-  next_sync_committee :: SyncCommittee
+  genesis_time_f :: u64
+  genesis_validators_root_f :: Hash256
+  slot_f :: Slot
+  fork_f :: Fork
+  latest_block_header_f :: BeaconBlockHeader
+  block_roots_f :: "Hash256 Vector"
+  state_roots_f :: "Hash256 Vector"
+  historical_roots_f :: "Hash256 List"
+  eth1_data_f :: Eth1Data
+  eth1_data_votes_f :: "Eth1Data List"
+  eth1_deposit_index_f :: u64
+  validators_f :: "Validator List"
+  balances_f :: "u64 List"
+  randao_mixes_f :: "Hash256 Vector"
+  slashings_f :: "u64 Vector"
+  previous_epoch_participation_f :: "ParticipationFlags List"
+  current_epoch_participation_f :: "ParticipationFlags List"
+  justification_bits_f :: Bitvector
+  previous_justified_checkpoint_f :: Checkpoint
+  current_justified_checkpoint_f :: Checkpoint
+  finalized_checkpoint_f :: Checkpoint
+  inactivity_scores_f :: "u64 List"
+  current_sync_committee_f :: SyncCommittee
+  next_sync_committee_f :: SyncCommittee
 
 end
