Utils.thy
@@ -12,8 +12,35 @@ definition enumerate :: "'a list \<Rightarrow> (u64 \<times> 'a) list" where
 definition safe_sum :: "u64 set \<Rightarrow> u64 option" where
   "safe_sum s \<equiv> foldl (\<lambda>acc x. acc \<bind> ((.+) x)) (Some (u64 0)) (sorted_list_of_set s)"
 
-(* FIXME(sproul): return optional value rather than undefined? *)
-definition list_index :: "'a List \<Rightarrow> u64 \<Rightarrow> 'a" where
-  "list_index l i \<equiv> list_inner l ! u64_to_nat i"
+definition list_index :: "'a List \<Rightarrow> u64 \<Rightarrow> 'a option" where
+  "list_index l i \<equiv>
+    if i < u64 (length (list_inner l)) then
+      Some (list_inner l ! u64_to_nat i)
+    else
+      None"
+
+definition unsafe_list_index :: "'a List \<Rightarrow> u64 \<Rightarrow> 'a" where
+  "unsafe_list_index l i \<equiv> the (list_index l i)"
+
+definition vector_index :: "'a Vector \<Rightarrow> u64 \<Rightarrow> 'a option" where
+  "vector_index v i \<equiv>
+    if i < u64 (length (vector_inner v)) then
+      Some (vector_inner v ! u64_to_nat i)
+    else
+      None"
+
+definition unsafe_vector_index :: "'a Vector \<Rightarrow> u64 \<Rightarrow> 'a" where
+  "unsafe_vector_index v i \<equiv> the (vector_index v i)"
+
+definition shift_and_clear_bitvector :: "Config \<Rightarrow> Bitvector \<Rightarrow> Bitvector" where
+  "shift_and_clear_bitvector c bv \<equiv>
+    Bitvector ([False] @ take (u64_to_nat (JUSTIFICATION_BITS_LENGTH c) - 1) (bitvector_inner bv))"
+
+definition bitvector_update :: "Bitvector \<Rightarrow> nat \<Rightarrow> bool \<Rightarrow> Bitvector" where
+  "bitvector_update bv i v \<equiv> Bitvector (list_update (bitvector_inner bv) i v)"
+
+definition bitvector_all :: "Bitvector \<Rightarrow> nat \<Rightarrow> nat \<Rightarrow> bool" where
+  "bitvector_all bv start end \<equiv>
+    list_all (\<lambda>x. x) (take (end - start) (drop start (bitvector_inner bv)))"
 
 end
